examples/test1_implicit.ml
@@ -1,0 +1,1808 @@
+
+type __ = Obj.t
+let __ = let rec f _ = Obj.repr f in Obj.repr f
+
+type 'a option =
+| Some of 'a
+| None
+
+(** val option_map : ('a1 -> 'a2) -> 'a1 option -> 'a2 option **)
+
+let option_map f = function
+| Some a -> Some (f a)
+| None -> None
+
+type ('a, 'b) sum =
+| Inl of 'a
+| Inr of 'b
+
+(** val app : 'a1 list -> 'a1 list -> 'a1 list **)
+
+let rec app l m =
+  match l with
+  | [] -> m
+  | a::l1 -> a::(app l1 m)
+
+type 'a sig0 = 'a
+  (* singleton inductive, whose constructor was exist *)
+
+type ('a, 'p) sigT =
+| ExistT of 'a * 'p
+
+type 'a sumor =
+| Inleft of 'a
+| Inright
+
+(** val add : int -> int -> int **)
+
+let rec add = ( + )
+
+(** val in_dec : ('a1 -> 'a1 -> bool) -> 'a1 -> 'a1 list -> bool **)
+
+let rec in_dec h a = function
+| [] -> false
+| y::l0 -> let s = h y a in if s then true else in_dec h a l0
+
+(** val map : ('a1 -> 'a2) -> 'a1 list -> 'a2 list **)
+
+let rec map f = function
+| [] -> []
+| a::t -> (f a)::(map f t)
+
+(** val fold_right : ('a2 -> 'a1 -> 'a1) -> 'a1 -> 'a2 list -> 'a1 **)
+
+let rec fold_right f a0 = function
+| [] -> a0
+| b::t -> f b (fold_right f a0 t)
+
+type 'configuration rEWRITING_SYSTEM =
+| Build_REWRITING_SYSTEM
+
+type ('label, 'configuration) lABELED_REWRITING_SYSTEM =
+| Build_LABELED_REWRITING_SYSTEM
+
+module type RED_MINI_LANG =
+ sig
+  type term
+
+  type ckind
+
+  type elem_context_kinded
+
+  val elem_plug : ckind -> ckind -> term -> elem_context_kinded -> term
+
+  type redex
+
+  type value
+
+  val value_to_term : ckind -> value -> term
+
+  val redex_to_term : ckind -> redex -> term
+
+  type context =
+  | Coq_empty
+  | Coq_ccons of ckind * ckind * elem_context_kinded * context
+
+  val context_rect :
+    ckind -> 'a1 -> (ckind -> ckind -> elem_context_kinded -> context -> 'a1 -> 'a1)
+    -> ckind -> context -> 'a1
+
+  val context_rec :
+    ckind -> 'a1 -> (ckind -> ckind -> elem_context_kinded -> context -> 'a1 -> 'a1)
+    -> ckind -> context -> 'a1
+
+  val compose : ckind -> ckind -> context -> ckind -> context -> context
+
+  val plug : term -> ckind -> ckind -> context -> term
+ end
+
+module RED_LANG_Facts =
+ functor (R:RED_MINI_LANG) ->
+ struct
+ end
+
+module type RED_MINI_LANG_WD =
+ sig
+  type term
+
+  type ckind
+
+  type elem_context_kinded
+
+  val elem_plug : ckind -> ckind -> term -> elem_context_kinded -> term
+
+  type redex
+
+  type value
+
+  val value_to_term : ckind -> value -> term
+
+  val redex_to_term : ckind -> redex -> term
+
+  type context =
+  | Coq_empty
+  | Coq_ccons of ckind * ckind * elem_context_kinded * context
+
+  val context_rect :
+    ckind -> 'a1 -> (ckind -> ckind -> elem_context_kinded -> context -> 'a1 -> 'a1)
+    -> ckind -> context -> 'a1
+
+  val context_rec :
+    ckind -> 'a1 -> (ckind -> ckind -> elem_context_kinded -> context -> 'a1 -> 'a1)
+    -> ckind -> context -> 'a1
+
+  val compose : ckind -> ckind -> context -> ckind -> context -> context
+
+  val plug : term -> ckind -> ckind -> context -> term
+
+  type decomp =
+  | Coq_d_red of ckind * redex * context
+  | Coq_d_val of value
+
+  val decomp_rect :
+    ckind -> (ckind -> redex -> context -> 'a1) -> (value -> 'a1) -> decomp -> 'a1
+
+  val decomp_rec :
+    ckind -> (ckind -> redex -> context -> 'a1) -> (value -> 'a1) -> decomp -> 'a1
+
+  val decomp_to_term : ckind -> decomp -> term
+ end
+
+module RedDecProcEqvDec =
+ functor (R:RED_MINI_LANG_WD) ->
+ struct
+  module RF = RED_LANG_Facts(R)
+ end
+
+module type RED_SEM =
+ sig
+  type term
+
+  type ckind
+
+  type elem_context_kinded
+
+  val elem_plug : ckind -> ckind -> term -> elem_context_kinded -> term
+
+  type redex
+
+  type value
+
+  val redex_to_term : ckind -> redex -> term
+
+  val value_to_term : ckind -> value -> term
+
+  val init_ckind : ckind
+
+  val contract : ckind -> redex -> term option
+
+  type context =
+  | Coq_empty
+  | Coq_ccons of ckind * ckind * elem_context_kinded * context
+
+  val context_rect :
+    ckind -> 'a1 -> (ckind -> ckind -> elem_context_kinded -> context -> 'a1 -> 'a1)
+    -> ckind -> context -> 'a1
+
+  val context_rec :
+    ckind -> 'a1 -> (ckind -> ckind -> elem_context_kinded -> context -> 'a1 -> 'a1)
+    -> ckind -> context -> 'a1
+
+  val plug : term -> ckind -> ckind -> context -> term
+
+  val compose : ckind -> ckind -> context -> ckind -> context -> context
+
+  type decomp =
+  | Coq_d_red of ckind * redex * context
+  | Coq_d_val of value
+
+  val decomp_rect :
+    ckind -> (ckind -> redex -> context -> 'a1) -> (value -> 'a1) -> decomp -> 'a1
+
+  val decomp_rec :
+    ckind -> (ckind -> redex -> context -> 'a1) -> (value -> 'a1) -> decomp -> 'a1
+
+  val decomp_to_term : ckind -> decomp -> term
+
+  val lrws : (ckind, term) lABELED_REWRITING_SYSTEM
+
+  val rws : term rEWRITING_SYSTEM
+ end
+
+module type PRE_REF_SEM =
+ sig
+  type term
+
+  type ckind
+
+  type elem_context_kinded
+
+  val elem_plug : ckind -> ckind -> term -> elem_context_kinded -> term
+
+  type redex
+
+  type value
+
+  val init_ckind : ckind
+
+  val value_to_term : ckind -> value -> term
+
+  val redex_to_term : ckind -> redex -> term
+
+  type context =
+  | Coq_empty
+  | Coq_ccons of ckind * ckind * elem_context_kinded * context
+
+  val context_rect :
+    ckind -> 'a1 -> (ckind -> ckind -> elem_context_kinded -> context -> 'a1 -> 'a1)
+    -> ckind -> context -> 'a1
+
+  val context_rec :
+    ckind -> 'a1 -> (ckind -> ckind -> elem_context_kinded -> context -> 'a1 -> 'a1)
+    -> ckind -> context -> 'a1
+
+  val compose : ckind -> ckind -> context -> ckind -> context -> context
+
+  val plug : term -> ckind -> ckind -> context -> term
+
+  type decomp =
+  | Coq_d_red of ckind * redex * context
+  | Coq_d_val of value
+
+  val decomp_rect :
+    ckind -> (ckind -> redex -> context -> 'a1) -> (value -> 'a1) -> decomp -> 'a1
+
+  val decomp_rec :
+    ckind -> (ckind -> redex -> context -> 'a1) -> (value -> 'a1) -> decomp -> 'a1
+
+  val decomp_to_term : ckind -> decomp -> term
+
+  val contract : ckind -> redex -> term option
+
+  val lrws : (ckind, term) lABELED_REWRITING_SYSTEM
+
+  val rws : term rEWRITING_SYSTEM
+ end
+
+module type RED_REF_SEM =
+ sig
+  module R :
+   RED_SEM
+
+  module ST :
+   sig
+    type elem_dec =
+    | Coq_ed_red of R.redex
+    | Coq_ed_dec of R.ckind * R.term * R.elem_context_kinded
+    | Coq_ed_val of R.value
+
+    val elem_dec_rect :
+      R.ckind -> (R.redex -> 'a1) -> (R.ckind -> R.term -> R.elem_context_kinded ->
+      'a1) -> (R.value -> 'a1) -> elem_dec -> 'a1
+
+    val elem_dec_rec :
+      R.ckind -> (R.redex -> 'a1) -> (R.ckind -> R.term -> R.elem_context_kinded ->
+      'a1) -> (R.value -> 'a1) -> elem_dec -> 'a1
+
+    val dec_term : R.term -> R.ckind -> elem_dec
+
+    val dec_context :
+      R.ckind -> R.ckind -> R.elem_context_kinded -> R.value -> elem_dec
+   end
+
+  type term = R.term
+
+  type ckind = R.ckind
+
+  type elem_context_kinded = R.elem_context_kinded
+
+  val elem_plug : ckind -> ckind -> term -> elem_context_kinded -> term
+
+  type redex = R.redex
+
+  type value = R.value
+
+  val redex_to_term : ckind -> redex -> term
+
+  val value_to_term : ckind -> value -> term
+
+  val init_ckind : ckind
+
+  val contract : ckind -> redex -> term option
+
+  type context = R.context =
+  | Coq_empty
+  | Coq_ccons of ckind * ckind * elem_context_kinded * context
+
+  val context_rect :
+    ckind -> 'a1 -> (ckind -> ckind -> elem_context_kinded -> context -> 'a1 -> 'a1)
+    -> ckind -> context -> 'a1
+
+  val context_rec :
+    ckind -> 'a1 -> (ckind -> ckind -> elem_context_kinded -> context -> 'a1 -> 'a1)
+    -> ckind -> context -> 'a1
+
+  val plug : term -> ckind -> ckind -> context -> term
+
+  val compose : ckind -> ckind -> context -> ckind -> context -> context
+
+  type decomp = R.decomp =
+  | Coq_d_red of ckind * redex * context
+  | Coq_d_val of value
+
+  val decomp_rect :
+    ckind -> (ckind -> redex -> context -> 'a1) -> (value -> 'a1) -> decomp -> 'a1
+
+  val decomp_rec :
+    ckind -> (ckind -> redex -> context -> 'a1) -> (value -> 'a1) -> decomp -> 'a1
+
+  val decomp_to_term : ckind -> decomp -> term
+
+  val lrws : (ckind, term) lABELED_REWRITING_SYSTEM
+
+  val rws : term rEWRITING_SYSTEM
+ end
+
+module RedRefSem =
+ functor (PR:PRE_REF_SEM) ->
+ functor (ST:sig
+  type elem_dec =
+  | Coq_ed_red of PR.redex
+  | Coq_ed_dec of PR.ckind * PR.term * PR.elem_context_kinded
+  | Coq_ed_val of PR.value
+
+  val elem_dec_rect :
+    PR.ckind -> (PR.redex -> 'a1) -> (PR.ckind -> PR.term -> PR.elem_context_kinded
+    -> 'a1) -> (PR.value -> 'a1) -> elem_dec -> 'a1
+
+  val elem_dec_rec :
+    PR.ckind -> (PR.redex -> 'a1) -> (PR.ckind -> PR.term -> PR.elem_context_kinded
+    -> 'a1) -> (PR.value -> 'a1) -> elem_dec -> 'a1
+
+  val dec_term : PR.term -> PR.ckind -> elem_dec
+
+  val dec_context :
+    PR.ckind -> PR.ckind -> PR.elem_context_kinded -> PR.value -> elem_dec
+
+  type elem_context_in =
+  | Coq_ec_in of PR.ckind * PR.elem_context_kinded
+
+  val elem_context_in_rect :
+    PR.ckind -> (PR.ckind -> PR.elem_context_kinded -> 'a1) -> elem_context_in -> 'a1
+
+  val elem_context_in_rec :
+    PR.ckind -> (PR.ckind -> PR.elem_context_kinded -> 'a1) -> elem_context_in -> 'a1
+
+  val ec_kinded_to_in :
+    PR.ckind -> PR.ckind -> PR.elem_context_kinded -> elem_context_in
+ end) ->
+ struct
+  module RLF = RED_LANG_Facts(PR)
+
+  module ST = ST
+
+  module R =
+   struct
+    type term = PR.term
+
+    type ckind = PR.ckind
+
+    type elem_context_kinded = PR.elem_context_kinded
+
+    (** val elem_plug : ckind -> ckind -> term -> elem_context_kinded -> term **)
+
+    let elem_plug =
+      PR.elem_plug
+
+    type redex = PR.redex
+
+    type value = PR.value
+
+    (** val init_ckind : ckind **)
+
+    let init_ckind =
+      PR.init_ckind
+
+    (** val value_to_term : ckind -> value -> term **)
+
+    let value_to_term =
+      PR.value_to_term
+
+    (** val redex_to_term : ckind -> redex -> term **)
+
+    let redex_to_term =
+      PR.redex_to_term
+
+    type context = PR.context =
+    | Coq_empty
+    | Coq_ccons of ckind * ckind * elem_context_kinded * context
+
+    (** val context_rect :
+        ckind -> 'a1 -> (ckind -> ckind -> elem_context_kinded -> context -> 'a1 ->
+        'a1) -> ckind -> context -> 'a1 **)
+
+    let rec context_rect k1 f f0 _ = function
+    | Coq_empty -> f
+    | Coq_ccons (k2, k3, ec, c0) -> f0 k2 k3 ec c0 (context_rect k1 f f0 k2 c0)
+
+    (** val context_rec :
+        ckind -> 'a1 -> (ckind -> ckind -> elem_context_kinded -> context -> 'a1 ->
+        'a1) -> ckind -> context -> 'a1 **)
+
+    let rec context_rec k1 f f0 _ = function
+    | Coq_empty -> f
+    | Coq_ccons (k2, k3, ec, c0) -> f0 k2 k3 ec c0 (context_rec k1 f f0 k2 c0)
+
+    (** val compose : ckind -> ckind -> context -> ckind -> context -> context **)
+
+    let rec compose k1 _ c0 k3 c1 =
+      match c0 with
+      | Coq_empty -> c1
+      | Coq_ccons (k2, k4, ec, c0') ->
+        Coq_ccons (k2, k4, ec, (compose k1 k2 c0' k3 c1))
+
+    (** val plug : term -> ckind -> ckind -> context -> term **)
+
+    let rec plug t k1 _ = function
+    | Coq_empty -> t
+    | Coq_ccons (k2, k3, ec, c') -> plug (elem_plug k2 k3 t ec) k1 k2 c'
+
+    type decomp = PR.decomp =
+    | Coq_d_red of ckind * redex * context
+    | Coq_d_val of value
+
+    (** val decomp_rect :
+        ckind -> (ckind -> redex -> context -> 'a1) -> (value -> 'a1) -> decomp ->
+        'a1 **)
+
+    let decomp_rect _ f f0 = function
+    | Coq_d_red (x0, x1, x2) -> f x0 x1 x2
+    | Coq_d_val x0 -> f0 x0
+
+    (** val decomp_rec :
+        ckind -> (ckind -> redex -> context -> 'a1) -> (value -> 'a1) -> decomp ->
+        'a1 **)
+
+    let decomp_rec _ f f0 = function
+    | Coq_d_red (x0, x1, x2) -> f x0 x1 x2
+    | Coq_d_val x0 -> f0 x0
+
+    (** val decomp_to_term : ckind -> decomp -> term **)
+
+    let decomp_to_term k = function
+    | Coq_d_red (k', r, c) -> plug (redex_to_term k' r) k k' c
+    | Coq_d_val v -> value_to_term k v
+
+    (** val contract : ckind -> redex -> term option **)
+
+    let contract =
+      PR.contract
+
+    (** val lrws : (ckind, term) lABELED_REWRITING_SYSTEM **)
+
+    let lrws =
+      Build_LABELED_REWRITING_SYSTEM
+
+    (** val rws : term rEWRITING_SYSTEM **)
+
+    let rws =
+      Build_REWRITING_SYSTEM
+   end
+
+  type term = PR.term
+
+  type ckind = PR.ckind
+
+  type elem_context_kinded = PR.elem_context_kinded
+
+  (** val elem_plug : ckind -> ckind -> term -> elem_context_kinded -> term **)
+
+  let elem_plug =
+    PR.elem_plug
+
+  type redex = PR.redex
+
+  type value = PR.value
+
+  (** val init_ckind : ckind **)
+
+  let init_ckind =
+    PR.init_ckind
+
+  (** val value_to_term : ckind -> value -> term **)
+
+  let value_to_term =
+    PR.value_to_term
+
+  (** val redex_to_term : ckind -> redex -> term **)
+
+  let redex_to_term =
+    PR.redex_to_term
+
+  type context = PR.context =
+  | Coq_empty
+  | Coq_ccons of ckind * ckind * elem_context_kinded * context
+
+  (** val context_rect :
+      ckind -> 'a1 -> (ckind -> ckind -> elem_context_kinded -> context -> 'a1 ->
+      'a1) -> ckind -> context -> 'a1 **)
+
+  let rec context_rect k1 f f0 _ = function
+  | Coq_empty -> f
+  | Coq_ccons (k2, k3, ec, c0) -> f0 k2 k3 ec c0 (context_rect k1 f f0 k2 c0)
+
+  (** val context_rec :
+      ckind -> 'a1 -> (ckind -> ckind -> elem_context_kinded -> context -> 'a1 ->
+      'a1) -> ckind -> context -> 'a1 **)
+
+  let rec context_rec k1 f f0 _ = function
+  | Coq_empty -> f
+  | Coq_ccons (k2, k3, ec, c0) -> f0 k2 k3 ec c0 (context_rec k1 f f0 k2 c0)
+
+  (** val compose : ckind -> ckind -> context -> ckind -> context -> context **)
+
+  let rec compose k1 _ c0 k3 c1 =
+    match c0 with
+    | Coq_empty -> c1
+    | Coq_ccons (k2, k4, ec, c0') ->
+      Coq_ccons (k2, k4, ec, (compose k1 k2 c0' k3 c1))
+
+  (** val plug : term -> ckind -> ckind -> context -> term **)
+
+  let rec plug t k1 _ = function
+  | Coq_empty -> t
+  | Coq_ccons (k2, k3, ec, c') -> plug (elem_plug k2 k3 t ec) k1 k2 c'
+
+  type decomp = PR.decomp =
+  | Coq_d_red of ckind * redex * context
+  | Coq_d_val of value
+
+  (** val decomp_rect :
+      ckind -> (ckind -> redex -> context -> 'a1) -> (value -> 'a1) -> decomp -> 'a1 **)
+
+  let decomp_rect _ f f0 = function
+  | Coq_d_red (x0, x1, x2) -> f x0 x1 x2
+  | Coq_d_val x0 -> f0 x0
+
+  (** val decomp_rec :
+      ckind -> (ckind -> redex -> context -> 'a1) -> (value -> 'a1) -> decomp -> 'a1 **)
+
+  let decomp_rec _ f f0 = function
+  | Coq_d_red (x0, x1, x2) -> f x0 x1 x2
+  | Coq_d_val x0 -> f0 x0
+
+  (** val decomp_to_term : ckind -> decomp -> term **)
+
+  let decomp_to_term k = function
+  | Coq_d_red (k', r, c) -> plug (redex_to_term k' r) k k' c
+  | Coq_d_val v -> value_to_term k v
+
+  (** val contract : ckind -> redex -> term option **)
+
+  let contract =
+    PR.contract
+
+  (** val lrws : (ckind, term) lABELED_REWRITING_SYSTEM **)
+
+  let lrws =
+    Build_LABELED_REWRITING_SYSTEM
+
+  (** val rws : term rEWRITING_SYSTEM **)
+
+  let rws =
+    Build_REWRITING_SYSTEM
+
+  module DPT = RedDecProcEqvDec(R)
+ end
+
+type 'a set = 'a list
+
+(** val internal_eq_rew_r_dep : 'a1 -> 'a1 -> 'a2 -> 'a2 **)
+
+let internal_eq_rew_r_dep _ _ hC =
+  hC
+
+(** val in_split_aux :
+    ('a1 -> 'a1 -> bool) -> 'a1 -> 'a1 set -> (('a1 set*'a1 set), __) sum **)
+
+let rec in_split_aux eq_A x0 = function
+| [] -> Inr __
+| y::l0 ->
+  let s = in_split_aux eq_A x0 l0 in
+  (match s with
+   | Inl s0 -> let x1,x2 = s0 in Inl ((y::x1),x2)
+   | Inr _ ->
+     if eq_A y x0
+     then internal_eq_rew_r_dep y x0 (fun _ _ _ -> Inl ([],l0)) __ __ __
+     else Inr __)
+
+(** val in_split :
+    ('a1 -> 'a1 -> bool) -> 'a1 -> 'a1 set -> ('a1 set, ('a1 set, __) sigT) sigT
+    sumor **)
+
+let in_split eq_A x0 l =
+  let hh = in_split_aux eq_A x0 l in
+  (match hh with
+   | Inl s -> let s0,s1 = s in Inleft (ExistT (s0, (ExistT (s1, __))))
+   | Inr _ -> Inright)
+
+type entropy (* AXIOM TO BE REALIZED *)
+
+module type DET_ABSTRACT_MACHINE =
+ sig
+  type term
+
+  type configuration
+
+  type value
+
+  val load : term -> configuration
+
+  val final : configuration -> value option
+
+  val next_conf : entropy -> configuration -> configuration option
+
+  val rws : configuration rEWRITING_SYSTEM
+
+  val dnext_conf : configuration -> configuration option
+ end
+
+module RefEvalApplyMachine =
+ functor (R:RED_REF_SEM) ->
+ struct
+  module RF = RED_LANG_Facts(R)
+
+  type term = R.term
+
+  type value = R.value
+
+  (** val value_to_term : value -> term **)
+
+  let value_to_term v =
+    R.value_to_term R.init_ckind v
+
+  type conf =
+  | Coq_c_eval of term * R.ckind * R.context
+  | Coq_c_apply of R.ckind * R.context * R.value
+
+  (** val conf_rect :
+      (term -> R.ckind -> R.context -> 'a1) -> (R.ckind -> R.context -> R.value ->
+      'a1) -> conf -> 'a1 **)
+
+  let conf_rect f f0 = function
+  | Coq_c_eval (x0, x1, x2) -> f x0 x1 x2
+  | Coq_c_apply (x0, x1, x2) -> f0 x0 x1 x2
+
+  (** val conf_rec :
+      (term -> R.ckind -> R.context -> 'a1) -> (R.ckind -> R.context -> R.value ->
+      'a1) -> conf -> 'a1 **)
+
+  let conf_rec f f0 = function
+  | Coq_c_eval (x0, x1, x2) -> f x0 x1 x2
+  | Coq_c_apply (x0, x1, x2) -> f0 x0 x1 x2
+
+  type configuration = conf
+
+  (** val load : term -> configuration **)
+
+  let load t =
+    Coq_c_eval (t, R.init_ckind, R.Coq_empty)
+
+  (** val value_to_conf : value -> configuration **)
+
+  let value_to_conf v =
+    Coq_c_apply (R.init_ckind, R.Coq_empty, v)
+
+  (** val final : configuration -> value option **)
+
+  let final = function
+  | Coq_c_eval (_, _, _) -> None
+  | Coq_c_apply (_, c0, v) ->
+    (match c0 with
+     | R.Coq_empty -> Some v
+     | R.Coq_ccons (_, _, _, _) -> None)
+
+  (** val decompile : configuration -> term **)
+
+  let decompile = function
+  | Coq_c_eval (t, k, c0) -> R.plug t R.init_ckind k c0
+  | Coq_c_apply (k, c0, v) -> R.plug (R.value_to_term k v) R.init_ckind k c0
+
+  (** val dnext_conf : configuration -> configuration option **)
+
+  let dnext_conf = function
+  | Coq_c_eval (t, k, c) ->
+    (match R.ST.dec_term t k with
+     | R.ST.Coq_ed_red r ->
+       option_map (fun t' -> Coq_c_eval (t', k, c)) (R.contract k r)
+     | R.ST.Coq_ed_dec (k', t0, ec) ->
+       Some (Coq_c_eval (t0, k', (R.Coq_ccons (k, k', ec, c))))
+     | R.ST.Coq_ed_val v -> Some (Coq_c_apply (k, c, v)))
+  | Coq_c_apply (_, c0, v) ->
+    (match c0 with
+     | R.Coq_empty -> None
+     | R.Coq_ccons (k2, k3, ec, c) ->
+       (match R.ST.dec_context k2 k3 ec v with
+        | R.ST.Coq_ed_red r ->
+          option_map (fun t' -> Coq_c_eval (t', k2, c)) (R.contract k2 r)
+        | R.ST.Coq_ed_dec (k', t, ec0) ->
+          Some (Coq_c_eval (t, k', (R.Coq_ccons (k2, k', ec0, c))))
+        | R.ST.Coq_ed_val v0 -> Some (Coq_c_apply (k2, c, v0))))
+
+  (** val next_conf : entropy -> configuration -> configuration option **)
+
+  let next_conf _ =
+    dnext_conf
+
+  (** val rws : configuration rEWRITING_SYSTEM **)
+
+  let rws =
+    Build_REWRITING_SYSTEM
+ end
+
+module DET_ABSTRACT_MACHINE_Facts =
+ functor (AM:DET_ABSTRACT_MACHINE) ->
+ struct
+ end
+
+module DetAbstractMachine_Sim =
+ functor (AM:DET_ABSTRACT_MACHINE) ->
+ struct
+  module AMF = DET_ABSTRACT_MACHINE_Facts(AM)
+
+  (** val n_steps : AM.configuration -> int -> AM.configuration option **)
+
+  let rec n_steps c n =
+    (fun fO fS n -> if n=0 then fO () else fS (n-1))
+      (fun _ -> Some c)
+      (fun n0 -> match AM.dnext_conf c with
+                 | Some c' -> n_steps c' n0
+                 | None -> None)
+      n
+ end
+
+module Lam_cbnd_PreRefSem =
+ struct
+  type id = int
+    (* singleton inductive, whose constructor was Id *)
+
+  (** val id_rect : (int -> 'a1) -> id -> 'a1 **)
+
+  let id_rect f =
+    f
+
+  (** val id_rec : (int -> 'a1) -> id -> 'a1 **)
+
+  let id_rec f =
+    f
+
+  type var = id
+
+  (** val eq_var : var -> var -> bool **)
+
+  let rec eq_var n y =
+    (fun fO fS n -> if n=0 then fO () else fS (n-1))
+      (fun _ ->
+      (fun fO fS n -> if n=0 then fO () else fS (n-1))
+        (fun _ -> true)
+        (fun _ -> false)
+        y)
+      (fun n0 ->
+      (fun fO fS n -> if n=0 then fO () else fS (n-1))
+        (fun _ -> false)
+        (fun m' -> eq_var n0 m')
+        y)
+      n
+
+  type vars = var set
+
+  type ck =
+  | E
+  | C
+
+  (** val ck_rect : 'a1 -> 'a1 -> ck -> 'a1 **)
+
+  let ck_rect f f0 = function
+  | E -> f
+  | C -> f0
+
+  (** val ck_rec : 'a1 -> 'a1 -> ck -> 'a1 **)
+
+  let ck_rec f f0 = function
+  | E -> f
+  | C -> f0
+
+  type ckvars =
+  | Coq_ckv of ck * vars
+
+  (** val ckvars_rect : (ck -> vars -> __ -> 'a1) -> ckvars -> 'a1 **)
+
+  let ckvars_rect f = function
+  | Coq_ckv (x0, x1) -> f x0 x1 __
+
+  (** val ckvars_rec : (ck -> vars -> __ -> 'a1) -> ckvars -> 'a1 **)
+
+  let ckvars_rec f = function
+  | Coq_ckv (x0, x1) -> f x0 x1 __
+
+  type ckind = ckvars
+
+  (** val fresh_for : vars -> var **)
+
+  let fresh_for xs =
+    add (succ 0) (fold_right add 0 (map (fun y -> y) xs))
+
+  type expr =
+  | App of expr * expr
+  | Var of var
+  | Lam of var * expr
+  | Let of var * expr * expr
+  | LetNd of var * expr * expr
+
+  (** val expr_rect :
+      (expr -> 'a1 -> expr -> 'a1 -> 'a1) -> (var -> 'a1) -> (var -> expr -> 'a1 ->
+      'a1) -> (var -> expr -> 'a1 -> expr -> 'a1 -> 'a1) -> (var -> expr -> 'a1 ->
+      expr -> 'a1 -> 'a1) -> expr -> 'a1 **)
+
+  let rec expr_rect f f0 f1 f2 f3 = function
+  | App (e0, e1) -> f e0 (expr_rect f f0 f1 f2 f3 e0) e1 (expr_rect f f0 f1 f2 f3 e1)
+  | Var v -> f0 v
+  | Lam (v, e0) -> f1 v e0 (expr_rect f f0 f1 f2 f3 e0)
+  | Let (v, e0, e1) ->
+    f2 v e0 (expr_rect f f0 f1 f2 f3 e0) e1 (expr_rect f f0 f1 f2 f3 e1)
+  | LetNd (v, e0, e1) ->
+    f3 v e0 (expr_rect f f0 f1 f2 f3 e0) e1 (expr_rect f f0 f1 f2 f3 e1)
+
+  (** val expr_rec :
+      (expr -> 'a1 -> expr -> 'a1 -> 'a1) -> (var -> 'a1) -> (var -> expr -> 'a1 ->
+      'a1) -> (var -> expr -> 'a1 -> expr -> 'a1 -> 'a1) -> (var -> expr -> 'a1 ->
+      expr -> 'a1 -> 'a1) -> expr -> 'a1 **)
+
+  let rec expr_rec f f0 f1 f2 f3 = function
+  | App (e0, e1) -> f e0 (expr_rec f f0 f1 f2 f3 e0) e1 (expr_rec f f0 f1 f2 f3 e1)
+  | Var v -> f0 v
+  | Lam (v, e0) -> f1 v e0 (expr_rec f f0 f1 f2 f3 e0)
+  | Let (v, e0, e1) ->
+    f2 v e0 (expr_rec f f0 f1 f2 f3 e0) e1 (expr_rec f f0 f1 f2 f3 e1)
+  | LetNd (v, e0, e1) ->
+    f3 v e0 (expr_rec f f0 f1 f2 f3 e0) e1 (expr_rec f f0 f1 f2 f3 e1)
+
+  type term = expr
+
+  type in_ctx =
+  | Coq_inctxVar of ck * var
+  | Coq_inctxApp_l of ck * var * in_ctx * expr
+  | Coq_inctxApp_r of ck * var * coq_struct * in_ctx
+  | Coq_inctxLam of var * var * in_ctx
+  | Coq_inctxSub of ck * var * var * in_ctx * expr
+  | Coq_inctxNdSub of ck * var * var * coq_struct * in_ctx
+  | Coq_inctxNdSub2 of ck * var * var * in_ctx * expr
+  and coq_struct =
+  | Coq_sVar of var
+  | Coq_sApp of coq_struct * normal
+  | Coq_sSub of var * expr * coq_struct
+  | Coq_sNdSub of var * coq_struct * coq_struct
+  and lambda_normal =
+  | Coq_lnfLam of var * normal
+  | Coq_lnfSub of var * expr * lambda_normal
+  | Coq_lnfNdSub of var * coq_struct * lambda_normal
+  and normal =
+  | Coq_nf_struct of coq_struct
+  | Coq_nf_lam_in_ctx of lambda_normal
+
+  (** val in_ctx_rect :
+      (ck -> var -> 'a1) -> (ck -> var -> var list -> __ -> in_ctx -> 'a1 -> expr ->
+      'a1) -> (ck -> var -> var list -> var list -> __ -> coq_struct -> in_ctx ->
+      'a1 -> 'a1) -> (var -> var -> vars -> __ -> in_ctx -> 'a1 -> 'a1) -> (ck ->
+      var -> var -> var list -> __ -> __ -> in_ctx -> 'a1 -> expr -> 'a1) -> (ck ->
+      var -> var -> var list -> vars -> __ -> __ -> coq_struct -> in_ctx -> 'a1 ->
+      'a1) -> (ck -> var -> vars -> var -> in_ctx -> 'a1 -> expr -> 'a1) -> ck ->
+      var -> vars -> in_ctx -> 'a1 **)
+
+  let rec in_ctx_rect f f0 f1 f2 f3 f4 f5 _ _ _ = function
+  | Coq_inctxVar (k, x0) -> f k x0
+  | Coq_inctxApp_l (k, x0, i0, e) ->
+    f0 k x0 __ (* 3rd argument (xs) of inctxApp_l *) __ i0
+      (in_ctx_rect f f0 f1 f2 f3 f4 f5 E x0 __ (* 3rd argument (xs) of inctxApp_l *)
+        i0) e
+  | Coq_inctxApp_r (k, x0, s, i0) ->
+    f1 k x0 __ (* 3rd argument (xs) of inctxApp_r *) __
+      (* 4th argument (ys) of inctxApp_r *) __ s i0
+      (in_ctx_rect f f0 f1 f2 f3 f4 f5 C x0 __ (* 3rd argument (xs) of inctxApp_r *)
+        i0)
+  | Coq_inctxLam (x0, y, i0) ->
+    f2 x0 y __ (* 3rd argument (xs) of inctxLam *) __ i0
+      (in_ctx_rect f f0 f1 f2 f3 f4 f5 C y __ (* 3rd argument (xs) of inctxLam *) i0)
+  | Coq_inctxSub (k, x0, y, i0, e) ->
+    f3 k x0 y __ (* 4th argument (xs) of inctxSub *) __ __ i0
+      (in_ctx_rect f f0 f1 f2 f3 f4 f5 k y __ (* 4th argument (xs) of inctxSub *) i0)
+      e
+  | Coq_inctxNdSub (k, x0, y, s, i0) ->
+    f4 k x0 y __ (* 4th argument (xs) of inctxNdSub *) __
+      (* 5th argument (zs) of inctxNdSub *) __ __ s i0
+      (in_ctx_rect f f0 f1 f2 f3 f4 f5 k y __ (* 5th argument (zs) of inctxNdSub *)
+        i0)
+  | Coq_inctxNdSub2 (k, y, v, i0, e) ->
+    f5 k y __ (* 3rd argument (xs) of inctxNdSub2 *) v i0
+      (in_ctx_rect f f0 f1 f2 f3 f4 f5 E y __ (* 3rd argument (xs) of inctxNdSub2 *)
+        i0) e
+
+  (** val in_ctx_rec :
+      (ck -> var -> 'a1) -> (ck -> var -> var list -> __ -> in_ctx -> 'a1 -> expr ->
+      'a1) -> (ck -> var -> var list -> var list -> __ -> coq_struct -> in_ctx ->
+      'a1 -> 'a1) -> (var -> var -> vars -> __ -> in_ctx -> 'a1 -> 'a1) -> (ck ->
+      var -> var -> var list -> __ -> __ -> in_ctx -> 'a1 -> expr -> 'a1) -> (ck ->
+      var -> var -> var list -> vars -> __ -> __ -> coq_struct -> in_ctx -> 'a1 ->
+      'a1) -> (ck -> var -> vars -> var -> in_ctx -> 'a1 -> expr -> 'a1) -> ck ->
+      var -> vars -> in_ctx -> 'a1 **)
+
+  let rec in_ctx_rec f f0 f1 f2 f3 f4 f5 _ _ _ = function
+  | Coq_inctxVar (k, x0) -> f k x0
+  | Coq_inctxApp_l (k, x0, i0, e) ->
+    f0 k x0 __ (* 3rd argument (xs) of inctxApp_l *) __ i0
+      (in_ctx_rec f f0 f1 f2 f3 f4 f5 E x0 __ (* 3rd argument (xs) of inctxApp_l *)
+        i0) e
+  | Coq_inctxApp_r (k, x0, s, i0) ->
+    f1 k x0 __ (* 3rd argument (xs) of inctxApp_r *) __
+      (* 4th argument (ys) of inctxApp_r *) __ s i0
+      (in_ctx_rec f f0 f1 f2 f3 f4 f5 C x0 __ (* 3rd argument (xs) of inctxApp_r *)
+        i0)
+  | Coq_inctxLam (x0, y, i0) ->
+    f2 x0 y __ (* 3rd argument (xs) of inctxLam *) __ i0
+      (in_ctx_rec f f0 f1 f2 f3 f4 f5 C y __ (* 3rd argument (xs) of inctxLam *) i0)
+  | Coq_inctxSub (k, x0, y, i0, e) ->
+    f3 k x0 y __ (* 4th argument (xs) of inctxSub *) __ __ i0
+      (in_ctx_rec f f0 f1 f2 f3 f4 f5 k y __ (* 4th argument (xs) of inctxSub *) i0)
+      e
+  | Coq_inctxNdSub (k, x0, y, s, i0) ->
+    f4 k x0 y __ (* 4th argument (xs) of inctxNdSub *) __
+      (* 5th argument (zs) of inctxNdSub *) __ __ s i0
+      (in_ctx_rec f f0 f1 f2 f3 f4 f5 k y __ (* 5th argument (zs) of inctxNdSub *)
+        i0)
+  | Coq_inctxNdSub2 (k, y, v, i0, e) ->
+    f5 k y __ (* 3rd argument (xs) of inctxNdSub2 *) v i0
+      (in_ctx_rec f f0 f1 f2 f3 f4 f5 E y __ (* 3rd argument (xs) of inctxNdSub2 *)
+        i0) e
+
+  (** val struct_rect :
+      (var -> 'a1) -> (vars -> vars -> coq_struct -> 'a1 -> normal -> 'a1) -> (var
+      -> var list -> __ -> expr -> coq_struct -> 'a1 -> 'a1) -> (var -> var set ->
+      vars -> var set -> __ -> __ -> __ -> coq_struct -> 'a1 -> coq_struct -> 'a1 ->
+      'a1) -> vars -> coq_struct -> 'a1 **)
+
+  let rec struct_rect f f0 f1 f2 _ = function
+  | Coq_sVar x0 -> f x0
+  | Coq_sApp (s0, n) ->
+    f0 __ (* 1st argument (xs) of sApp *) __ (* 2nd argument (ys) of sApp *) s0
+      (struct_rect f f0 f1 f2 __ (* 1st argument (xs) of sApp *) s0) n
+  | Coq_sSub (x0, e, s0) ->
+    f1 x0 __ (* 2nd argument (ys) of sSub *) __ e s0
+      (struct_rect f f0 f1 f2 __ (* 2nd argument (ys) of sSub *) s0)
+  | Coq_sNdSub (x0, s0, s1) ->
+    f2 x0 __ (* 2nd argument (ys) of sNdSub *) __ (* 3rd argument (zs) of sNdSub *)
+      __ (* 4th argument (xs) of sNdSub *) __ __ __ s0
+      (struct_rect f f0 f1 f2 __ (* 3rd argument (zs) of sNdSub *) s0) s1
+      (struct_rect f f0 f1 f2 __ (* 4th argument (xs) of sNdSub *) s1)
+
+  (** val struct_rec :
+      (var -> 'a1) -> (vars -> vars -> coq_struct -> 'a1 -> normal -> 'a1) -> (var
+      -> var list -> __ -> expr -> coq_struct -> 'a1 -> 'a1) -> (var -> var set ->
+      vars -> var set -> __ -> __ -> __ -> coq_struct -> 'a1 -> coq_struct -> 'a1 ->
+      'a1) -> vars -> coq_struct -> 'a1 **)
+
+  let rec struct_rec f f0 f1 f2 _ = function
+  | Coq_sVar x0 -> f x0
+  | Coq_sApp (s0, n) ->
+    f0 __ (* 1st argument (xs) of sApp *) __ (* 2nd argument (ys) of sApp *) s0
+      (struct_rec f f0 f1 f2 __ (* 1st argument (xs) of sApp *) s0) n
+  | Coq_sSub (x0, e, s0) ->
+    f1 x0 __ (* 2nd argument (ys) of sSub *) __ e s0
+      (struct_rec f f0 f1 f2 __ (* 2nd argument (ys) of sSub *) s0)
+  | Coq_sNdSub (x0, s0, s1) ->
+    f2 x0 __ (* 2nd argument (ys) of sNdSub *) __ (* 3rd argument (zs) of sNdSub *)
+      __ (* 4th argument (xs) of sNdSub *) __ __ __ s0
+      (struct_rec f f0 f1 f2 __ (* 3rd argument (zs) of sNdSub *) s0) s1
+      (struct_rec f f0 f1 f2 __ (* 4th argument (xs) of sNdSub *) s1)
+
+  (** val lambda_normal_rect :
+      (var -> vars -> normal -> 'a1) -> (var -> var list -> __ -> expr ->
+      lambda_normal -> 'a1 -> 'a1) -> (var -> var set -> vars -> var set -> __ -> __
+      -> __ -> coq_struct -> lambda_normal -> 'a1 -> 'a1) -> vars -> lambda_normal
+      -> 'a1 **)
+
+  let rec lambda_normal_rect f f0 f1 _ = function
+  | Coq_lnfLam (x0, n) -> f x0 __ (* 2nd argument (xs) of lnfLam *) n
+  | Coq_lnfSub (x0, e, l0) ->
+    f0 x0 __ (* 2nd argument (ys) of lnfSub *) __ e l0
+      (lambda_normal_rect f f0 f1 __ (* 2nd argument (ys) of lnfSub *) l0)
+  | Coq_lnfNdSub (x0, s, l0) ->
+    f1 x0 __ (* 2nd argument (ys) of lnfNdSub *) __
+      (* 3rd argument (zs) of lnfNdSub *) __ (* 4th argument (xs) of lnfNdSub *) __
+      __ __ s l0
+      (lambda_normal_rect f f0 f1 __ (* 4th argument (xs) of lnfNdSub *) l0)
+
+  (** val lambda_normal_rec :
+      (var -> vars -> normal -> 'a1) -> (var -> var list -> __ -> expr ->
+      lambda_normal -> 'a1 -> 'a1) -> (var -> var set -> vars -> var set -> __ -> __
+      -> __ -> coq_struct -> lambda_normal -> 'a1 -> 'a1) -> vars -> lambda_normal
+      -> 'a1 **)
+
+  let rec lambda_normal_rec f f0 f1 _ = function
+  | Coq_lnfLam (x0, n) -> f x0 __ (* 2nd argument (xs) of lnfLam *) n
+  | Coq_lnfSub (x0, e, l0) ->
+    f0 x0 __ (* 2nd argument (ys) of lnfSub *) __ e l0
+      (lambda_normal_rec f f0 f1 __ (* 2nd argument (ys) of lnfSub *) l0)
+  | Coq_lnfNdSub (x0, s, l0) ->
+    f1 x0 __ (* 2nd argument (ys) of lnfNdSub *) __
+      (* 3rd argument (zs) of lnfNdSub *) __ (* 4th argument (xs) of lnfNdSub *) __
+      __ __ s l0
+      (lambda_normal_rec f f0 f1 __ (* 4th argument (xs) of lnfNdSub *) l0)
+
+  (** val normal_rect :
+      (vars -> coq_struct -> 'a1) -> (vars -> lambda_normal -> 'a1) -> vars ->
+      normal -> 'a1 **)
+
+  let normal_rect f f0 _ = function
+  | Coq_nf_struct x0 -> f __ (* 1st argument (xs) of nf_struct *) x0
+  | Coq_nf_lam_in_ctx x0 -> f0 __ (* 1st argument (xs) of nf_lam_in_ctx *) x0
+
+  (** val normal_rec :
+      (vars -> coq_struct -> 'a1) -> (vars -> lambda_normal -> 'a1) -> vars ->
+      normal -> 'a1 **)
+
+  let normal_rec f f0 _ = function
+  | Coq_nf_struct x0 -> f __ (* 1st argument (xs) of nf_struct *) x0
+  | Coq_nf_lam_in_ctx x0 -> f0 __ (* 1st argument (xs) of nf_lam_in_ctx *) x0
+
+  type sub =
+  | Coq_subMt
+  | Coq_subCons of var * expr * sub
+
+  (** val sub_rect : 'a1 -> (var -> expr -> sub -> 'a1 -> 'a1) -> sub -> 'a1 **)
+
+  let rec sub_rect f f0 = function
+  | Coq_subMt -> f
+  | Coq_subCons (v, e, s0) -> f0 v e s0 (sub_rect f f0 s0)
+
+  (** val sub_rec : 'a1 -> (var -> expr -> sub -> 'a1 -> 'a1) -> sub -> 'a1 **)
+
+  let rec sub_rec f f0 = function
+  | Coq_subMt -> f
+  | Coq_subCons (v, e, s0) -> f0 v e s0 (sub_rec f f0 s0)
+
+  type sub_ext =
+  | Coq_subSimple of sub
+  | Coq_subNd of var * expr * sub_ext
+
+  (** val sub_ext_rect :
+      (sub -> 'a1) -> (var -> expr -> sub_ext -> 'a1 -> 'a1) -> sub_ext -> 'a1 **)
+
+  let rec sub_ext_rect f f0 = function
+  | Coq_subSimple s0 -> f s0
+  | Coq_subNd (v, e, s0) -> f0 v e s0 (sub_ext_rect f f0 s0)
+
+  (** val sub_ext_rec :
+      (sub -> 'a1) -> (var -> expr -> sub_ext -> 'a1 -> 'a1) -> sub_ext -> 'a1 **)
+
+  let rec sub_ext_rec f f0 = function
+  | Coq_subSimple s0 -> f s0
+  | Coq_subNd (v, e, s0) -> f0 v e s0 (sub_ext_rec f f0 s0)
+
+  (** val sub_to_term : sub -> term -> term **)
+
+  let rec sub_to_term s t =
+    match s with
+    | Coq_subMt -> t
+    | Coq_subCons (x0, r, s') -> Let (x0, r, (sub_to_term s' t))
+
+  (** val sub_ext_to_term : sub_ext -> term -> term **)
+
+  let rec sub_ext_to_term s t =
+    match s with
+    | Coq_subSimple s0 -> sub_to_term s0 t
+    | Coq_subNd (x0, r, s') -> LetNd (x0, r, (sub_ext_to_term s' t))
+
+  (** val struct_to_term : vars -> coq_struct -> term **)
+
+  let rec struct_to_term _ = function
+  | Coq_sVar x0 -> Var x0
+  | Coq_sApp (s0, n) ->
+    App ((struct_to_term __ (* 1st argument (xs) of sApp *) s0), (normal_to_term n))
+  | Coq_sSub (x0, e, s0) ->
+    Let (x0, e, (struct_to_term __ (* 2nd argument (ys) of sSub *) s0))
+  | Coq_sNdSub (x0, s0, sx) ->
+    LetNd (x0, (struct_to_term __ (* 3rd argument (zs) of sNdSub *) s0),
+      (struct_to_term __ (* 4th argument (xs) of sNdSub *) sx))
+
+  (** val lambda_normal_to_term : vars -> lambda_normal -> term **)
+
+  and lambda_normal_to_term _ = function
+  | Coq_lnfLam (x0, n0) -> Lam (x0, (normal_to_term n0))
+  | Coq_lnfSub (x0, e, n0) ->
+    Let (x0, e, (lambda_normal_to_term __ (* 2nd argument (ys) of lnfSub *) n0))
+  | Coq_lnfNdSub (x0, s, n0) ->
+    LetNd (x0, (struct_to_term __ (* 3rd argument (zs) of lnfNdSub *) s),
+      (lambda_normal_to_term __ (* 4th argument (xs) of lnfNdSub *) n0))
+
+  (** val normal_to_term : normal -> term **)
+
+  and normal_to_term = function
+  | Coq_nf_struct s -> struct_to_term __ (* 1st argument (xs) of nf_struct *) s
+  | Coq_nf_lam_in_ctx ln ->
+    lambda_normal_to_term __ (* 1st argument (xs) of nf_lam_in_ctx *) ln
+
+  (** val nf_to_term : ck -> var -> in_ctx -> term **)
+
+  let rec nf_to_term _ _ = function
+  | Coq_inctxVar (_, x0) -> Var x0
+  | Coq_inctxApp_l (_, x0, n, e) -> App ((nf_to_term E x0 n), e)
+  | Coq_inctxApp_r (_, x0, s, neu') ->
+    App ((struct_to_term __ (* 4th argument (ys) of inctxApp_r *) s),
+      (nf_to_term C x0 neu'))
+  | Coq_inctxLam (x0, y, neu') -> Lam (x0, (nf_to_term C y neu'))
+  | Coq_inctxSub (k, x0, y, n, e) -> Let (x0, e, (nf_to_term k y n))
+  | Coq_inctxNdSub (k, x0, y, s, n) ->
+    LetNd (x0, (struct_to_term __ (* 4th argument (xs) of inctxNdSub *) s),
+      (nf_to_term k y n))
+  | Coq_inctxNdSub2 (_, y, x0, ny, nx) -> LetNd (x0, (nf_to_term E y ny), nx)
+
+  (** val struct_to_normal : coq_struct -> normal **)
+
+  let struct_to_normal s =
+    Coq_nf_struct s
+
+  type coq_val =
+  | Coq_vCLam of lambda_normal
+  | Coq_vStruct of ck * coq_struct
+  | Coq_vNeu of ck * var * in_ctx
+  | Coq_vELam of var * term * sub
+
+  (** val val_rect :
+      (var set -> var list -> __ -> __ -> lambda_normal -> 'a1) -> (ck -> var set ->
+      var list -> __ -> __ -> coq_struct -> 'a1) -> (ck -> var set -> var -> var
+      list -> __ -> __ -> __ -> in_ctx -> 'a1) -> (var list -> __ -> var -> term ->
+      sub -> 'a1) -> ckind -> coq_val -> 'a1 **)
+
+  let val_rect f f0 f1 f2 _ = function
+  | Coq_vCLam x0 ->
+    f __ (* 1st argument (xs) of vCLam *) __ (* 2nd argument (ys) of vCLam *) __ __
+      x0
+  | Coq_vStruct (x0, x1) ->
+    f0 x0 __ (* 2nd argument (xs) of vStruct *) __
+      (* 3rd argument (ys) of vStruct *) __ __ x1
+  | Coq_vNeu (x0, x1, x2) ->
+    f1 x0 __ (* 2nd argument (xs) of vNeu *) x1 __ (* 4th argument (ys) of vNeu *)
+      __ __ __ x2
+  | Coq_vELam (x0, x1, x2) -> f2 __ (* 1st argument (xs) of vELam *) __ x0 x1 x2
+
+  (** val val_rec :
+      (var set -> var list -> __ -> __ -> lambda_normal -> 'a1) -> (ck -> var set ->
+      var list -> __ -> __ -> coq_struct -> 'a1) -> (ck -> var set -> var -> var
+      list -> __ -> __ -> __ -> in_ctx -> 'a1) -> (var list -> __ -> var -> term ->
+      sub -> 'a1) -> ckind -> coq_val -> 'a1 **)
+
+  let val_rec f f0 f1 f2 _ = function
+  | Coq_vCLam x0 ->
+    f __ (* 1st argument (xs) of vCLam *) __ (* 2nd argument (ys) of vCLam *) __ __
+      x0
+  | Coq_vStruct (x0, x1) ->
+    f0 x0 __ (* 2nd argument (xs) of vStruct *) __
+      (* 3rd argument (ys) of vStruct *) __ __ x1
+  | Coq_vNeu (x0, x1, x2) ->
+    f1 x0 __ (* 2nd argument (xs) of vNeu *) x1 __ (* 4th argument (ys) of vNeu *)
+      __ __ __ x2
+  | Coq_vELam (x0, x1, x2) -> f2 __ (* 1st argument (xs) of vELam *) __ x0 x1 x2
+
+  type value = coq_val
+
+  (** val val_to_term : ckind -> coq_val -> term **)
+
+  let rec val_to_term _ = function
+  | Coq_vCLam n -> lambda_normal_to_term __ (* 1st argument (xs) of vCLam *) n
+  | Coq_vStruct (_, s) -> struct_to_term __ (* 2nd argument (xs) of vStruct *) s
+  | Coq_vNeu (k, x0, n) -> nf_to_term k x0 n
+  | Coq_vELam (x0, t, s) -> sub_to_term s (Lam (x0, t))
+
+  (** val value_to_term : ckind -> coq_val -> term **)
+
+  let value_to_term =
+    val_to_term
+
+  type red =
+  | Coq_rApp of ck * var * term * sub * term
+  | Coq_rSub of ck * var * term * var * term * sub
+  | Coq_rSubNd of ck * var * in_ctx * term
+  | Coq_rSubWrong of ck * var * coq_struct * coq_struct
+  | Coq_rSubWrong2 of var * coq_struct * lambda_normal
+  | Coq_rSubNdE of var * coq_struct * var * term * sub
+
+  (** val red_rect :
+      (ck -> var list -> __ -> var -> term -> sub -> term -> 'a1) -> (ck -> var ->
+      var list -> __ -> term -> var -> term -> sub -> 'a1) -> (ck -> var -> var set
+      -> var list -> __ -> __ -> in_ctx -> term -> 'a1) -> (ck -> var -> var set ->
+      var list -> var set -> __ -> __ -> __ -> __ -> coq_struct -> coq_struct ->
+      'a1) -> (var -> var set -> var list -> var set -> __ -> __ -> __ -> __ ->
+      coq_struct -> lambda_normal -> 'a1) -> (var -> var set -> var list -> __ -> __
+      -> coq_struct -> var -> term -> sub -> 'a1) -> ckind -> red -> 'a1 **)
+
+  let red_rect f f0 f1 f2 f3 f4 _ = function
+  | Coq_rApp (x0, x1, x2, x3, x4) ->
+    f x0 __ (* 2nd argument (xs) of rApp *) __ x1 x2 x3 x4
+  | Coq_rSub (x0, x1, x2, x3, x4, x5) ->
+    f0 x0 x1 __ (* 3rd argument (xs) of rSub *) __ x2 x3 x4 x5
+  | Coq_rSubNd (x0, x1, x2, x3) ->
+    f1 x0 x1 __ (* 3rd argument (xs) of rSubNd *) __
+      (* 4th argument (ys) of rSubNd *) __ __ x2 x3
+  | Coq_rSubWrong (x0, x1, x2, x3) ->
+    f2 x0 x1 __ (* 3rd argument (xs) of rSubWrong *) __
+      (* 4th argument (ys) of rSubWrong *) __ (* 5th argument (zs) of rSubWrong *)
+      __ __ __ __ x2 x3
+  | Coq_rSubWrong2 (x0, x1, x2) ->
+    f3 x0 __ (* 2nd argument (xs) of rSubWrong2 *) __
+      (* 3rd argument (ys) of rSubWrong2 *) __ (* 4th argument (zs) of rSubWrong2 *)
+      __ __ __ __ x1 x2
+  | Coq_rSubNdE (x0, x1, x2, x3, x4) ->
+    f4 x0 __ (* 2nd argument (xs) of rSubNdE *) __
+      (* 3rd argument (ys) of rSubNdE *) __ __ x1 x2 x3 x4
+
+  (** val red_rec :
+      (ck -> var list -> __ -> var -> term -> sub -> term -> 'a1) -> (ck -> var ->
+      var list -> __ -> term -> var -> term -> sub -> 'a1) -> (ck -> var -> var set
+      -> var list -> __ -> __ -> in_ctx -> term -> 'a1) -> (ck -> var -> var set ->
+      var list -> var set -> __ -> __ -> __ -> __ -> coq_struct -> coq_struct ->
+      'a1) -> (var -> var set -> var list -> var set -> __ -> __ -> __ -> __ ->
+      coq_struct -> lambda_normal -> 'a1) -> (var -> var set -> var list -> __ -> __
+      -> coq_struct -> var -> term -> sub -> 'a1) -> ckind -> red -> 'a1 **)
+
+  let red_rec f f0 f1 f2 f3 f4 _ = function
+  | Coq_rApp (x0, x1, x2, x3, x4) ->
+    f x0 __ (* 2nd argument (xs) of rApp *) __ x1 x2 x3 x4
+  | Coq_rSub (x0, x1, x2, x3, x4, x5) ->
+    f0 x0 x1 __ (* 3rd argument (xs) of rSub *) __ x2 x3 x4 x5
+  | Coq_rSubNd (x0, x1, x2, x3) ->
+    f1 x0 x1 __ (* 3rd argument (xs) of rSubNd *) __
+      (* 4th argument (ys) of rSubNd *) __ __ x2 x3
+  | Coq_rSubWrong (x0, x1, x2, x3) ->
+    f2 x0 x1 __ (* 3rd argument (xs) of rSubWrong *) __
+      (* 4th argument (ys) of rSubWrong *) __ (* 5th argument (zs) of rSubWrong *)
+      __ __ __ __ x2 x3
+  | Coq_rSubWrong2 (x0, x1, x2) ->
+    f3 x0 __ (* 2nd argument (xs) of rSubWrong2 *) __
+      (* 3rd argument (ys) of rSubWrong2 *) __ (* 4th argument (zs) of rSubWrong2 *)
+      __ __ __ __ x1 x2
+  | Coq_rSubNdE (x0, x1, x2, x3, x4) ->
+    f4 x0 __ (* 2nd argument (xs) of rSubNdE *) __
+      (* 3rd argument (ys) of rSubNdE *) __ __ x1 x2 x3 x4
+
+  type redex = red
+
+  (** val redex_to_term : ckind -> redex -> term **)
+
+  let redex_to_term _ = function
+  | Coq_rApp (_, x0, t, s, t') -> App ((sub_to_term s (Lam (x0, t))), t')
+  | Coq_rSub (_, x0, n, y, t, s) -> LetNd (x0, (sub_to_term s (Lam (y, t))), n)
+  | Coq_rSubNd (k, x0, n, t) -> Let (x0, t, (nf_to_term k x0 n))
+  | Coq_rSubWrong (_, x0, s, s1) ->
+    LetNd (x0, (normal_to_term (struct_to_normal s)),
+      (normal_to_term (struct_to_normal s1)))
+  | Coq_rSubWrong2 (x0, s, s1) ->
+    LetNd (x0, (normal_to_term (struct_to_normal s)),
+      (lambda_normal_to_term __ (* 4th argument (zs) of rSubWrong2 *) s1))
+  | Coq_rSubNdE (x0, s, y, t, s0) ->
+    LetNd (x0, (normal_to_term (struct_to_normal s)), (sub_to_term s0 (Lam (y, t))))
+
+  (** val subst : var -> term -> term -> term **)
+
+  let rec subst x0 s t = match t with
+  | App (t1, t2) -> App ((subst x0 s t1), (subst x0 s t2))
+  | Var x' -> if eq_var x0 x' then s else t
+  | Lam (x', t1) -> Lam (x', (if eq_var x0 x' then t1 else subst x0 s t1))
+  | Let (x', r, u) ->
+    Let (x', (subst x0 s r), (if eq_var x0 x' then u else subst x0 s u))
+  | LetNd (x1, r, n) ->
+    LetNd (x1, (subst x0 s r), (if eq_var x0 x1 then n else subst x0 s n))
+
+  type eck =
+  | Coq_k_lam_c of var list * var
+  | Coq_k_ap_r of var list * ck * term
+  | Coq_k_ap_l_E of ck * coq_struct
+  | Coq_in_let of ck * var * term
+  | Coq_let_var of ck * var list * var * expr
+  | Coq_let_var2 of ck * var * coq_struct
+
+  (** val eck_rect :
+      (var list -> var -> __ -> __ -> 'a1) -> (var list -> ck -> __ -> term -> 'a1)
+      -> (ck -> var list -> var set -> __ -> __ -> coq_struct -> 'a1) -> (ck -> var
+      list -> var -> __ -> __ -> term -> 'a1) -> (ck -> var list -> var -> __ ->
+      expr -> 'a1) -> (ck -> var -> var set -> var list -> __ -> __ -> __ ->
+      coq_struct -> 'a1) -> ckind -> ckind -> eck -> 'a1 **)
+
+  let eck_rect f f0 f1 f2 f3 f4 _ _ = function
+  | Coq_k_lam_c (x0, x1) -> f x0 x1 __ __
+  | Coq_k_ap_r (x0, x1, x2) -> f0 x0 x1 __ x2
+  | Coq_k_ap_l_E (x0, x1) ->
+    f1 x0 __ (* 2nd argument (xs) of k_ap_l_E *) __
+      (* 3rd argument (ys) of k_ap_l_E *) __ __ x1
+  | Coq_in_let (x0, x1, x2) -> f2 x0 __ (* 2nd argument (xs) of in_let *) x1 __ __ x2
+  | Coq_let_var (x0, x1, x2, x3) -> f3 x0 x1 x2 __ x3
+  | Coq_let_var2 (x0, x1, x2) ->
+    f4 x0 x1 __ (* 3rd argument (xs) of let_var2 *) __
+      (* 4th argument (ys) of let_var2 *) __ __ __ x2
+
+  (** val eck_rec :
+      (var list -> var -> __ -> __ -> 'a1) -> (var list -> ck -> __ -> term -> 'a1)
+      -> (ck -> var list -> var set -> __ -> __ -> coq_struct -> 'a1) -> (ck -> var
+      list -> var -> __ -> __ -> term -> 'a1) -> (ck -> var list -> var -> __ ->
+      expr -> 'a1) -> (ck -> var -> var set -> var list -> __ -> __ -> __ ->
+      coq_struct -> 'a1) -> ckind -> ckind -> eck -> 'a1 **)
+
+  let eck_rec f f0 f1 f2 f3 f4 _ _ = function
+  | Coq_k_lam_c (x0, x1) -> f x0 x1 __ __
+  | Coq_k_ap_r (x0, x1, x2) -> f0 x0 x1 __ x2
+  | Coq_k_ap_l_E (x0, x1) ->
+    f1 x0 __ (* 2nd argument (xs) of k_ap_l_E *) __
+      (* 3rd argument (ys) of k_ap_l_E *) __ __ x1
+  | Coq_in_let (x0, x1, x2) -> f2 x0 __ (* 2nd argument (xs) of in_let *) x1 __ __ x2
+  | Coq_let_var (x0, x1, x2, x3) -> f3 x0 x1 x2 __ x3
+  | Coq_let_var2 (x0, x1, x2) ->
+    f4 x0 x1 __ (* 3rd argument (xs) of let_var2 *) __
+      (* 4th argument (ys) of let_var2 *) __ __ __ x2
+
+  type elem_context_kinded = eck
+
+  (** val init_ckind : ckind **)
+
+  let init_ckind =
+    Coq_ckv (C, [])
+
+  (** val elem_plug : ckind -> ckind -> term -> elem_context_kinded -> term **)
+
+  let elem_plug _ _ t = function
+  | Coq_k_lam_c (_, x0) -> Lam (x0, t)
+  | Coq_k_ap_r (_, _, tr) -> App (t, tr)
+  | Coq_k_ap_l_E (_, s) -> App ((normal_to_term (struct_to_normal s)), t)
+  | Coq_in_let (_, x0, s) -> Let (x0, s, t)
+  | Coq_let_var (_, _, x0, s) -> LetNd (x0, t, s)
+  | Coq_let_var2 (_, x0, s) -> LetNd (x0, (normal_to_term (struct_to_normal s)), t)
+
+  type context =
+  | Coq_empty
+  | Coq_ccons of ckind * ckind * elem_context_kinded * context
+
+  (** val context_rect :
+      ckind -> 'a1 -> (ckind -> ckind -> elem_context_kinded -> context -> 'a1 ->
+      'a1) -> ckind -> context -> 'a1 **)
+
+  let rec context_rect k1 f f0 _ = function
+  | Coq_empty -> f
+  | Coq_ccons (k2, k3, ec, c0) -> f0 k2 k3 ec c0 (context_rect k1 f f0 k2 c0)
+
+  (** val context_rec :
+      ckind -> 'a1 -> (ckind -> ckind -> elem_context_kinded -> context -> 'a1 ->
+      'a1) -> ckind -> context -> 'a1 **)
+
+  let rec context_rec k1 f f0 _ = function
+  | Coq_empty -> f
+  | Coq_ccons (k2, k3, ec, c0) -> f0 k2 k3 ec c0 (context_rec k1 f f0 k2 c0)
+
+  (** val compose : ckind -> ckind -> context -> ckind -> context -> context **)
+
+  let rec compose k1 _ c0 k3 c1 =
+    match c0 with
+    | Coq_empty -> c1
+    | Coq_ccons (k2, k4, ec, c0') ->
+      Coq_ccons (k2, k4, ec, (compose k1 k2 c0' k3 c1))
+
+  (** val plug : term -> ckind -> ckind -> context -> term **)
+
+  let rec plug t k1 _ = function
+  | Coq_empty -> t
+  | Coq_ccons (k2, k3, ec, c') -> plug (elem_plug k2 k3 t ec) k1 k2 c'
+
+  (** val contract : ckind -> redex -> term option **)
+
+  let contract _ = function
+  | Coq_rApp (_, x0, r0, s, t) -> Some (sub_to_term s (Let (x0, t, r0)))
+  | Coq_rSub (_, x0, n, y, t, s) -> Some (subst x0 (sub_to_term s (Lam (y, t))) n)
+  | Coq_rSubNd (k, x0, n, e) -> Some (LetNd (x0, e, (nf_to_term k x0 n)))
+  | Coq_rSubNdE (x0, s, y, t, s0) ->
+    Some (Let (x0, (normal_to_term (struct_to_normal s)),
+      (sub_to_term s0 (Lam (y, t)))))
+  | _ -> None
+
+  type decomp =
+  | Coq_d_red of ckind * redex * context
+  | Coq_d_val of value
+
+  (** val decomp_rect :
+      ckind -> (ckind -> redex -> context -> 'a1) -> (value -> 'a1) -> decomp -> 'a1 **)
+
+  let decomp_rect _ f f0 = function
+  | Coq_d_red (x0, x1, x2) -> f x0 x1 x2
+  | Coq_d_val x0 -> f0 x0
+
+  (** val decomp_rec :
+      ckind -> (ckind -> redex -> context -> 'a1) -> (value -> 'a1) -> decomp -> 'a1 **)
+
+  let decomp_rec _ f f0 = function
+  | Coq_d_red (x0, x1, x2) -> f x0 x1 x2
+  | Coq_d_val x0 -> f0 x0
+
+  (** val decomp_to_term : ckind -> decomp -> term **)
+
+  let decomp_to_term k = function
+  | Coq_d_red (k', r, c) -> plug (redex_to_term k' r) k k' c
+  | Coq_d_val v -> value_to_term k v
+
+  (** val lrws : (ckind, term) lABELED_REWRITING_SYSTEM **)
+
+  let lrws =
+    Build_LABELED_REWRITING_SYSTEM
+
+  (** val rws : term rEWRITING_SYSTEM **)
+
+  let rws =
+    Build_REWRITING_SYSTEM
+ end
+
+open Lam_cbnd_PreRefSem
+   
+module Lam_cbn_Strategy =
+ struct
+  type elem_dec =
+  | Coq_ed_red of redex
+  | Coq_ed_dec of ckind * term
+     * elem_context_kinded
+  | Coq_ed_val of value
+
+  (** val elem_dec_rect :
+      ckind -> (redex -> 'a1) ->
+      (ckind -> term ->
+      elem_context_kinded -> 'a1) -> (value ->
+      'a1) -> elem_dec -> 'a1 **)
+
+  let elem_dec_rect _ f f0 f1 = function
+  | Coq_ed_red x0 -> f x0
+  | Coq_ed_dec (x0, x1, x2) -> f0 x0 x1 x2
+  | Coq_ed_val x0 -> f1 x0
+
+  (** val elem_dec_rec :
+      ckind -> (redex -> 'a1) ->
+      (ckind -> term ->
+      elem_context_kinded -> 'a1) -> (value ->
+      'a1) -> elem_dec -> 'a1 **)
+
+  let elem_dec_rec _ f f0 f1 = function
+  | Coq_ed_red x0 -> f x0
+  | Coq_ed_dec (x0, x1, x2) -> f0 x0 x1 x2
+  | Coq_ed_val x0 -> f1 x0
+
+  (** val dec_term :
+      term -> ckind -> elem_dec **)
+
+  let dec_term t = function
+  | Coq_ckv (c, xs) ->
+    (match c with
+     | E ->
+       (match t with
+        | App (t1, t2) ->
+          Coq_ed_dec ((Coq_ckv (E, xs)), t1,
+            (Coq_k_ap_r (xs, E, t2)))
+        | Var x0 ->
+          if in_dec eq_var x0 xs
+          then Coq_ed_val (Coq_vStruct (E,
+                 (Coq_sVar x0)))
+          else Coq_ed_val (Coq_vNeu (E, x0,
+                 (Coq_inctxVar (E, x0))))
+        | Lam (x0, t1) ->
+          Coq_ed_val (Coq_vELam (x0, t1,
+            Coq_subMt))
+        | Let (x0, t1, t2) ->
+          if in_dec eq_var x0 xs
+          then let f = fresh_for xs in
+               Coq_ed_dec ((Coq_ckv (E, xs)),
+               (subst x0 (Var f) t2),
+               (Coq_in_let (E, f, t1)))
+          else Coq_ed_dec ((Coq_ckv (E, xs)),
+                 t2, (Coq_in_let (E, x0, t1)))
+        | LetNd (x0, t0, n) ->
+          Coq_ed_dec ((Coq_ckv (E, xs)), t0,
+            (Coq_let_var (E, xs, x0, n))))
+     | C ->
+       (match t with
+        | App (t1, t2) ->
+          Coq_ed_dec ((Coq_ckv (E, xs)), t1,
+            (Coq_k_ap_r (xs, C, t2)))
+        | Var x0 ->
+          if in_dec eq_var x0 xs
+          then Coq_ed_val (Coq_vStruct (C,
+                 (Coq_sVar x0)))
+          else Coq_ed_val (Coq_vNeu (C, x0,
+                 (Coq_inctxVar (C, x0))))
+        | Lam (x0, t1) ->
+          if in_dec eq_var x0 xs
+          then let f = fresh_for xs in
+               Coq_ed_dec ((Coq_ckv (C,
+               (f::xs))),
+               (subst x0 (Var f) t1),
+               (Coq_k_lam_c (xs, f)))
+          else Coq_ed_dec ((Coq_ckv (C,
+                 (x0::xs))), t1, (Coq_k_lam_c (xs, x0)))
+        | Let (x0, t1, t2) ->
+          if in_dec eq_var x0 xs
+          then let f = fresh_for xs in
+               Coq_ed_dec ((Coq_ckv (C, xs)),
+               (subst x0 (Var f) t2),
+               (Coq_in_let (C, f, t1)))
+          else Coq_ed_dec ((Coq_ckv (C, xs)),
+                 t2, (Coq_in_let (C, x0, t1)))
+        | LetNd (x0, t0, n) ->
+          Coq_ed_dec ((Coq_ckv (E, xs)), t0,
+            (Coq_let_var (C, xs, x0, n)))))
+
+  (** val dec_context :
+      ckind -> ckind ->
+      elem_context_kinded -> value -> elem_dec **)
+
+  let dec_context _ _ ec v =
+    match ec with
+    | Coq_k_lam_c (xs, x0) ->
+      (match v with
+       | Coq_vCLam l ->
+         Coq_ed_val (Coq_vCLam (Coq_lnfLam
+           (x0, (Coq_nf_lam_in_ctx l))))
+       | Coq_vStruct (k0, s) ->
+         (match k0 with
+          | E -> assert false (* absurd case *)
+          | C ->
+            Coq_ed_val (Coq_vCLam (Coq_lnfLam
+              (x0, (Coq_nf_struct s)))))
+       | Coq_vNeu (k0, y, c) ->
+         (match k0 with
+          | E -> assert false (* absurd case *)
+          | C ->
+            if eq_var x0 y
+            then Coq_ed_dec ((Coq_ckv (C,
+                   (x0::xs))),
+                   (nf_to_term C y c),
+                   (Coq_k_lam_c (xs, x0)))
+            else Coq_ed_val (Coq_vNeu (C, y,
+                   (Coq_inctxLam (x0, y, c)))))
+       | Coq_vELam (_, _, _) -> assert false (* absurd case *))
+    | Coq_k_ap_r (xs, k0, t) ->
+      (match v with
+       | Coq_vCLam _ -> assert false (* absurd case *)
+       | Coq_vStruct (k1, s) ->
+         (match k1 with
+          | E ->
+            Coq_ed_dec ((Coq_ckv (C, xs)), t,
+              (Coq_k_ap_l_E (k0, s)))
+          | C -> assert false (* absurd case *))
+       | Coq_vNeu (k1, x0, c) ->
+         (match k1 with
+          | E ->
+            Coq_ed_val (Coq_vNeu (k0, x0,
+              (Coq_inctxApp_l (k0, x0, c, t))))
+          | C -> assert false (* absurd case *))
+       | Coq_vELam (x0, t0, s) ->
+         Coq_ed_red (Coq_rApp (k0, x0, t0, s, t)))
+    | Coq_k_ap_l_E (k0, s) ->
+      (match v with
+       | Coq_vCLam l ->
+         Coq_ed_val (Coq_vStruct (k0,
+           (Coq_sApp (s, (Coq_nf_lam_in_ctx
+           l)))))
+       | Coq_vStruct (k1, s1) ->
+         (match k1 with
+          | E -> assert false (* absurd case *)
+          | C ->
+            Coq_ed_val (Coq_vStruct (k0,
+              (Coq_sApp (s,
+              (struct_to_normal s1))))))
+       | Coq_vNeu (k1, x0, c) ->
+         (match k1 with
+          | E -> assert false (* absurd case *)
+          | C ->
+            Coq_ed_val (Coq_vNeu (k0, x0,
+              (Coq_inctxApp_r (k0, x0, s, c)))))
+       | Coq_vELam (_, _, _) -> assert false (* absurd case *))
+    | Coq_in_let (k0, x0, t) ->
+      (match k0 with
+       | E ->
+         (match v with
+          | Coq_vCLam _ -> assert false (* absurd case *)
+          | Coq_vStruct (k1, s) ->
+            (match k1 with
+             | E ->
+               Coq_ed_val (Coq_vStruct (E,
+                 (Coq_sSub (x0, t, s))))
+             | C -> assert false (* absurd case *))
+          | Coq_vNeu (_, y, c) ->
+            if eq_var x0 y
+            then Coq_ed_red (Coq_rSubNd (E, y,
+                   c, t))
+            else Coq_ed_val (Coq_vNeu (E, y,
+                   (Coq_inctxSub (E, x0, y, c,
+                   t))))
+          | Coq_vELam (y, r, s) ->
+            Coq_ed_val (Coq_vELam (y, r,
+              (Coq_subCons (x0, t, s)))))
+       | C ->
+         (match v with
+          | Coq_vCLam ln ->
+            Coq_ed_val (Coq_vCLam (Coq_lnfSub
+              (x0, t, ln)))
+          | Coq_vStruct (k1, s) ->
+            (match k1 with
+             | E -> assert false (* absurd case *)
+             | C ->
+               Coq_ed_val (Coq_vStruct (C,
+                 (Coq_sSub (x0, t, s)))))
+          | Coq_vNeu (_, y, c) ->
+            if eq_var x0 y
+            then Coq_ed_red (Coq_rSubNd (C, y,
+                   c, t))
+            else Coq_ed_val (Coq_vNeu (C, y,
+                   (Coq_inctxSub (C, x0, y, c,
+                   t))))
+          | Coq_vELam (_, _, _) -> assert false (* absurd case *)))
+    | Coq_let_var (k, xs, x0, t) ->
+      (match v with
+       | Coq_vCLam _ -> assert false (* absurd case *)
+       | Coq_vStruct (k0, s) ->
+         (match k0 with
+          | E ->
+            (match in_split eq_var x0 xs with
+             | Inleft s2 ->
+               let ExistT (x1, s3) = s2 in
+               let ExistT (x2, _) = s3 in
+               let f = fresh_for (app x1 (x0::x2)) in
+               Coq_ed_dec ((Coq_ckv (k, (f::(app x1 (x0::x2))))),
+               (subst x0 (Var f) t),
+               (Coq_let_var2 (k, f, s)))
+             | Inright ->
+               Coq_ed_dec ((Coq_ckv (k, (x0::xs))), t,
+                 (Coq_let_var2 (k, x0, s))))
+          | C -> assert false (* absurd case *))
+       | Coq_vNeu (k0, y, c) ->
+         (match k0 with
+          | E ->
+            Coq_ed_val (Coq_vNeu (k, y,
+              (Coq_inctxNdSub2 (k, y, x0, c, t))))
+          | C -> assert false (* absurd case *))
+       | Coq_vELam (y, r, s) ->
+         Coq_ed_red (Coq_rSub (k, x0, t, y, r, s)))
+    | Coq_let_var2 (k0, x0, s1) ->
+      (match k0 with
+       | E ->
+         (match v with
+          | Coq_vCLam _ -> assert false (* absurd case *)
+          | Coq_vStruct (k1, s) ->
+            (match k1 with
+             | E -> Coq_ed_val (Coq_vStruct (E, (Coq_sNdSub (x0, s1, s))))
+ (*              let hh =
+                 in_split eq_var x0 __
+                   (* 2nd argument (xs) of vStruct *)
+               in
+               (match hh with
+                | Inleft _ ->
+                  Coq_ed_val (Coq_vStruct (E,
+                    (Coq_sNdSub (x0, s1, s))))
+                | Inright ->
+                  Coq_ed_red (Coq_rSubWrong
+                    (E, x0, s1, s)))*)
+             | C -> assert false (* absurd case *) )
+          | Coq_vNeu (_, y, c) ->
+            Coq_ed_val
+              (let val0 = Coq_inctxNdSub (E,
+                 x0, y, s1, c)
+               in
+               Coq_vNeu (E, y, val0))
+          | Coq_vELam (y, r, s) ->
+            Coq_ed_red (Coq_rSubNdE (x0, s1, y, r, s)))
+       | C ->
+         (match v with
+          | Coq_vCLam nl -> let vv = Coq_lnfNdSub (x0, s1, nl) in
+               Coq_ed_val (Coq_vCLam vv)
+(*            let s4 =
+              in_split eq_var x0 __
+                (* 1st argument (xs) of vCLam *)
+            in
+            (match s4 with
+             | Inleft _ ->
+               let vv = Coq_lnfNdSub (x0, s1, nl) in
+               Coq_ed_val (Coq_vCLam vv)
+             | Inright -> Coq_ed_red (Coq_rSubWrong2 (x0, s1, nl))) *)
+          | Coq_vStruct (k1, s) ->
+            (match k1 with
+             | E -> assert false (* absurd case *)
+             | C -> Coq_ed_val (Coq_vStruct (C,
+                    (Coq_sNdSub (x0, s1, s)))))
+(*               (match in_split eq_var x0 __
+                        (* 2nd argument (xs) of vStruct *) with
+                | Inleft _ ->
+                  Coq_ed_val (Coq_vStruct (C,
+                    (Coq_sNdSub (x0, s1, s))))
+                | Inright ->
+                  Coq_ed_red (Coq_rSubWrong
+                    (C, x0, s1, s)))) *)
+          | Coq_vNeu (_, y, c) ->
+            Coq_ed_val
+              (let val0 = Coq_inctxNdSub (C,
+                 x0, y, s1, c)
+               in
+               Coq_vNeu (C, y, val0))
+          | Coq_vELam (_, _, _) -> assert false (* absurd case *)))
+
+  type elem_context_in =
+  | Coq_ec_in of ckind * elem_context_kinded
+
+  (** val elem_context_in_rect :
+      ckind -> (ckind ->
+      elem_context_kinded -> 'a1) -> elem_context_in -> 'a1 **)
+
+  let elem_context_in_rect _ f = function
+  | Coq_ec_in (x0, x1) -> f x0 x1
+
+  (** val elem_context_in_rec :
+      ckind -> (ckind ->
+      elem_context_kinded -> 'a1) -> elem_context_in -> 'a1 **)
+
+  let elem_context_in_rec _ f = function
+  | Coq_ec_in (x0, x1) -> f x0 x1
+
+  (** val ec_kinded_to_in :
+      ckind -> ckind ->
+      elem_context_kinded -> elem_context_in **)
+
+  let ec_kinded_to_in _ k2 ec =
+    Coq_ec_in (k2, ec)
+ end
+
+module Lam_cbn_RefSem = RedRefSem(Lam_cbnd_PreRefSem)(Lam_cbn_Strategy)
+
+module Lam_cbn_EAM = RefEvalApplyMachine(Lam_cbn_RefSem)
+
+module Lam_cbn_sim = DetAbstractMachine_Sim(Lam_cbn_EAM)
+
+open Lam_cbn_RefSem      
+open Lam_cbn_EAM
+open Lam_cbn_sim
+   
+(** val x : id **)
+
+let x =
+  succ 0
+
+(** val id0 : expr **)
+
+let id0 =
+  Lam (x, (Var x))
+
+(** val list_configs :
+    Lam_cbn_EAM.configuration option -> int -> int ->
+    (int*Lam_cbn_EAM.configuration) list **)
+
+let rec list_configs c n i =
+  (fun fO fS n -> if n=0 then fO () else fS (n-1))
+    (fun _ -> [])
+    (fun n' ->
+    match c with
+    | Some c' -> (i,c')::(list_configs (Lam_cbn_sim.n_steps c' (succ 0)) n' (succ i))
+    | None -> [])
+    n
+
+(** val list_configurations :
+    Lam_cbn_EAM.term -> int -> (int*Lam_cbn_EAM.configuration) list **)
+
+let rec list_configurations t n =
+  list_configs (Some (Lam_cbn_EAM.load t)) n (succ 0)
+
+(** val test1 : (int*Lam_cbn_EAM.configuration) list **)
+
+let test1 =
+  list_configurations id0 (succ (succ (succ (succ (succ (succ (succ (succ (succ
+    (succ (succ (succ (succ (succ (succ (succ (succ (succ (succ (succ (succ (succ
+    (succ (succ (succ (succ (succ (succ (succ (succ (succ (succ (succ (succ (succ
+    (succ (succ (succ (succ (succ (succ (succ (succ (succ (succ (succ (succ (succ
+    (succ (succ 0))))))))))))))))))))))))))))))))))))))))))))))))))
